More debug option to solve pred + Refactor test

apps/tc/tc/stdpp/inj_test.v
@@ -1,67 +1,57 @@
 From elpi.apps.tc Require Import compiler.
 From Coq Require Export Morphisms RelationClasses List Bool Setoid Peano Utf8.
-
-Class Inj {A B} (R : relation A) (S : relation B) (f : A -> B) : Prop :=
-  inj x y : S (f x) (f y) -> R x y.
-Elpi Override TC TC_check Inj.
 Require Import Lia.
 
 Generalizable All Variables.
 
-Definition g x := x + 1.
-Definition f (x: nat) := x.
+(* Elpi Debug "debug" "debug ctx->clause" "show-tc-test".  *)
+
+Class Inj {A B} (R : relation A) (S : relation B) (f : A -> B) :=
+  inj x y : S (f x) (f y) -> R x y.
+Elpi Override TC TC_check Inj.
+
+Class Inj2 {A B C} (R1 : relation A) (R2 : relation B)
+    (S : relation C) (f : A → B → C) : Prop :=
+  inj2 x1 x2 y1 y2 : S (f x1 x2) (f y1 y2) → R1 x1 y1 ∧ R2 x2 y2.
+
+Local Instance ffff: Inj eq eq (PeanoNat.Nat.succ). Admitted.
+
+Elpi add_instances Inj. 
+Check (_ : Inj _ _ PeanoNat.Nat.succ).
+Check (_ : Inj _ _ S).
+
+Definition gInj x := x + 1.
+Definition fInj (x: nat) := x.
 
 Axiom eq1 : relation nat.
 Axiom eq2 : relation nat.
 Axiom eq3 : relation nat.
 
-Lemma isInjg : Inj eq3 eq1 g. Admitted.
+Local Instance isInjg : Inj eq3 eq1 gInj. Admitted.
 
-Lemma isInjf : Inj eq1 eq3 f. Admitted.
+Local Instance isInjf : Inj eq1 eq3 fInj. Admitted.
 
-Lemma isInjf_old : Inj eq1 eq2 f. Admitted.
-Lemma isInjg_old : Inj eq2 eq3 g. Admitted.
+Local Instance isInjf_old : Inj eq1 eq2 fInj. Admitted.
+Local Instance isInjg_old : Inj eq2 eq3 gInj. Admitted.
 
-Lemma isInjinr {A B}: Inj eq eq (@inr A B).
-Proof.
-  red; intros.
-  injection H.
-  easy.
-Qed.
+Lemma isInjinr {A B}: Inj eq eq (@inr A B). Admitted.
 
-Lemma isInjf_eq : Inj eq eq f.
-Proof. red; intuition. Defined.
+Local Instance isInjf_eq : Inj eq eq fInj. Admitted.
+Local Instance isInjg_eq : Inj eq eq gInj. Admitted.
 
-Lemma isInjg_eq : Inj eq eq g.
-Proof. red; unfold g; intros [| x] [|y]; lia. Defined.
-
-Global Existing Instance isInjf_eq.
-Global Existing Instance isInjg_eq.
-Global Existing Instance isInjf.
-Global Existing Instance isInjg.
-Global Existing Instance isInjf_old.
-Global Existing Instance isInjg_old.
-Local Instance id_inj {A} : Inj eq eq (@id A).
-Admitted.
-Local Instance inl_inj {A B} : Inj eq eq (@inl A B).
-Admitted.
-Local Instance inr_inj {A B} : Inj eq eq (@inr A B).
-Admitted.
+Local Instance id_inj {A} : Inj eq eq (@id A). Admitted.
+Local Instance inl_inj {A B} : Inj eq eq (@inl A B). Admitted.
+Local Instance inr_inj {A B} : Inj eq eq (@inr A B). Admitted.
 
 Definition compose {T1 T2 T3: Type} (g: T2 -> T3) (f : T1 -> T2) (x: T1) := g(f x).
 Local Instance compose_inj {A B C} R1 R2 R3 (f : A -> B) (g : B -> C) :
   Inj R1 R2 f -> Inj R2 R3 g -> Inj R1 R3 (compose g f).
 Admitted.
 
-Elpi add_instances "instances" isInjf_eq isInjg_eq.
-Elpi Print TC_check.
-(* Elpi add_instances Inj. *)
-
-Check (_ : Inj _ _ (compose g f)).
-
 Elpi add_instances Inj.
 
-(* Elpi Debug "debug" "debug ctx->clause" "show-tc-test".  *)
+Check (_ : Inj _ _ S).
+Check (_ : Inj _ _ (compose gInj fInj)).
 
 Goal forall (T1 T2 : Type) (f: T1 -> T2) (x : bool), 
   let r := Inj eq eq f in 
@@ -70,7 +60,8 @@ Goal forall (T1 T2 : Type) (f: T1 -> T2) (x : bool),
   intros.
   simpl in H.
   Check (_ : Inj _ _ f).
-Admitted.
+  apply _.
+Qed.
 
 Goal forall (T1 T2 : Type) (f: T1 -> T2), 
   let r := Inj eq eq f in 
@@ -84,12 +75,13 @@ Goal forall (T1 T2 : Type) (f: T1 -> T2),
   simpl in H.
   unfold r in H.
   Check (_ : Inj _ _ f).
-Admitted.
+  apply _.
+Qed.
 
 Section testInj.
   Context (f : nat -> nat -> nat) `{!Inj eq eq f}.
 
-  Local Instance xxx : Inj eq eq (compose f (Nat.add 3)).
+  Global Instance xxx : Inj eq eq (compose f (Nat.add 3)).
   Admitted.
 
   Elpi add_instances Inj.
@@ -100,9 +92,50 @@ End testInj.
 
 Elpi Print TC_check.
 
-Class Inj2 {A B C} (R1 : relation A) (R2 : relation B)
-    (S : relation C) (f : A → B → C) : Prop :=
-  inj2 x1 x2 y1 y2 : S (f x1 x2) (f y1 y2) → R1 x1 y1 ∧ R2 x2 y2.
+Print Instances Inj.
+
+Elpi Accumulate TC_check lp:{{
+  pred def2let i:goal-ctx, o:term.
+  def2let [decl _Var _Name Ty] (Ty).
+  def2let [(def _ Name Ty Body)| TL] (let Name Ty Body (x\ TLT)) :-
+    def2let TL TLT.
+  def2let [decl _Var _Name Ty | TL] (app [Ty, TLT]) :-
+    def2let TL TLT.
+  def2let _ _:- coq.say "not ehre", fail.
+
+  :after "hintHook"
+  solve (goal Ctx _ Ty Sol _ as G) GL :-
+    var Sol,
+    % Add's the section's definition to the current context
+    % in order to add its TC if present
+    std.map {coq.env.section} (x\r\ sigma F\ coq.env.typeof (const x) F, r = (decl (global (const x)) _ F)) SectionCtx,
+    ctx->clause {std.append Ctx SectionCtx} Clauses,
+    % coq.say Ctx "\n",
+    % std.rev Ctx CtxRev,
+    % def2let CtxRev RClauses,
+    % @redflags! coq.redflags.zeta => coq.reduction.lazy.norm RClauses Y,
+    % coq.say "ACCA" RClauses,
+    % coq.say "BlaBB" Y,
+    Clauses => if (tc Ty X) 
+      (
+        refine X G GL ; 
+        coq.say "illtyped solution:" {coq.term->string X}
+      ) 
+      (GL = [seal G]).
+
+}}.
+Elpi Typecheck TC_check.
+
+(* Elpi Query TC_check lp:{{
+  X = {{let x := 1 in let y := 2 in let z := 3 in x}},
+  @redflags! coq.redflags.zeta => coq.reduction.lazy.norm X Y,
+  coq.say Y.
+}}. *)
+
+Goal let x := 1 in let y := 2 in let z := 3 in x = x -> Inj eq eq (Nat.mul 0) -> Inj eq eq (Nat.mul 0).
+  intros.
+  apply _.
+Qed.
 
 Local Instance inj2_inj_1 `{Inj2 A B C R1 R2 R3 ff} y : Inj R1 R3 (λ x, ff x y).
 Admitted.
@@ -110,107 +143,69 @@ Admitted.
 Global Instance inj2_inj_2 `{Inj2 A B C R1 R2 R3 ff} x : Inj R2 R3 (ff x).
 Admitted.
 
-Elpi Accumulate TC_check lp:{{
-  :before "hintHook"
-  solve (goal Ctx _ Ty Sol _ as G) GL :-
-    var Sol,
-    % Add's the section's definition to the current context
-    % in order to add its TC if present
-    std.map {coq.env.section} (x\r\ sigma F\ coq.env.typeof (const x) F, r = (decl (global (const x)) _ F)) SectionCtx,
-    ctx->clause {std.append Ctx SectionCtx} Clauses,
-    Clauses => if (tc Ty X) 
-      (
-        refine X G GL ; 
-        coq.say "illtyped solution:" {coq.term->string X}
-      ) 
-      (GL = [seal G]).
-}}.
-Elpi Typecheck TC_check.
+Elpi add_instances Inj.
 
-Elpi Accumulate tc.db lp:{{
-  :after "complexHook"
-  tc {{ Inj _ _ lp:{{app L}} }} S :- 
-    L = [_, _, _ | _],
-    std.last L Last,
-    std.drop-last 1 L Firsts,
-    tc {{Inj _ _ lp:{{app [app Firsts, Last]}}}} S.
-}}.
-Elpi Typecheck TC_check.
+(* Elpi Print TC_check. *)
 
-Elpi add_instances Inj Inj2.
-Elpi Typecheck TC_check.
-
-Goal Inj2 eq eq eq Nat.add -> Inj eq eq (Nat.add 0).
-intros.
-apply _.
+Goal Inj2 eq eq eq Nat.mul -> Inj eq eq (Nat.mul 0).
+  intros.
+  apply _.
 Qed.
-
-Generalizable All Variables.
-Class Equiv A := equiv: relation A.
 
 Goal Inj2 eq eq eq Nat.add -> Inj eq eq (fun x => Nat.add x 0).
 intros.
 apply _.
 Qed.
 
-(* Elpi Accumulate TC_check lp:{{
-  :before "hintHook"
-  tc A B :-
-    coq.say "A" A "B" B "End", fail.
- }}.
-Elpi Typecheck TC_check. *)
-
-(* Elpi Accumulate tc.db lp:{{
-  :after "complexHook"
-  tc {{ Inj _ _ lp:{{app L}} }} S :- 
-    L = [_, _, _ | _],
+Elpi Accumulate tc.db lp:{{
+  % :before "hintHook"
+  tc {{ @Inj lp:T1 lp:T2 lp:R1 lp:R3 lp:{{app L}} }} S :- 
     std.last L Last,
+    coq.typecheck Last Ty ok,
     std.drop-last 1 L Firsts,
-    S = {{@inj2_inj_2 _ _ _ _ _ _ lp:{app Firsts} _ lp:Last}}.
-}}.
-Elpi Typecheck TC_check. *)
-
-
-(* Elpi Accumulate tc.db lp:{{
-  pred prod-len i:term, o:int.
-  prod-len (prod _ _ E) R :-
-    pi x\ sigma X\ prod-len (E x) X, R is X + 1.
-  prod-len _ 1.
-  pred give-len i:term.
-  give-len (prod Name Ty Cnt) :-
-    prod-len Ty Len,
-    coq.say Name Len,
-    pi x\ give-len (Cnt x).
-  give-len _.
-
-  pred compile2 i:term, i:term, i:list (list prop), i:list term, o:prop.
-  compile2 (prod _ T F) CT ListRHS ListVar (pi x\ C x) :-
-    prod-len T Len,
-    coq.say Len,
-    pi p\ sigma L\
-
-      compile2 (F p) CT L [p | ListVar] (C p).
-  compile2 _ I ListRHS ListVar (tc Ty AppInst :- RevRHS) :- 
-    AppInst = app [I | {std.rev ListVar}],
-    std.rev ListRHS RevRHS.
-}}.
-Elpi Typecheck TC_check. *)
-
-Elpi Query TC_check lp:{{
-  coq.locate "Inj" X,
-  const C = X,
-  coq.env.const C _ R.
-  % give-len R.
-}}.
+    if (Firsts = [F]) true (F = app Firsts),
+    S = {{@inj2_inj_2 _ _ _ _ _ _ lp:F lp:S1 lp:Last}},
+    tc {{ @Inj2 lp:Ty lp:T1 lp:T2 _ lp:R1 lp:R3 lp:F }} S1.
+  }}.
+Elpi Typecheck TC_check.
 
 Definition p (T : Type) := @pair T T.
+Elpi add_instances Inj.
 
-Elpi Print TC_check.
-Goal forall (T1 T2: Set), Inj2 eq eq eq (@p nat) -> Inj eq eq (@p nat 0).
-intros.
-(* apply (inj2_inj_2 ). *)
+Elpi Accumulate TC_check lp:{{
+  :before "hintHook"
+  tc A _ :- coq.say "A" A, fail.
+}}.
+Elpi Typecheck TC_check.
+
+Goal Inj eq eq (compose fInj gInj).
 apply _.
 Qed.
+
+Elpi Accumulate tc.db lp:{{
+  tc {{ Inj lp:R1 lp:R3 lp:F }} S :- 
+    F = (fun _ _ _), !,
+    G = {{ compose _ _ }},
+    coq.unify-eq G F ok,
+    tc {{ Inj lp:R1 lp:R3 lp:G }} S.
+}}.
+
+Check (_ : Inj _ _ (compose fInj gInj)).
+Check (_ : Inj _ _ (fun x => fInj (gInj x))). 
+
+Goal forall (T1 T2: Set), Inj2 eq eq eq (@pair nat T1) -> Inj eq eq (@pair nat T1 0).
+intros.
+apply _.
+(* apply (inj2_inj_2 ). *)
+Qed.
+
+Goal forall (A: Type) (x: A -> A), let y := Inj eq eq x in let z := y in z -> Inj eq eq (compose x x).
+Proof.
+  intros T x y z H.
+  (* apply _. *)
+  (* following diverges: the compiler should unfold the def *)
+  (* Check (_ : Inj eq eq (compose x x)). *)
+Admitted. 
 
 (* Global Hint Mode Inj - - ! ! -: typeclass_instances.
 Global Hint Mode Inj - - ! ! !: typeclass_instances. *)
@@ -221,10 +216,3 @@ Global Hint Mode Inj - - ! ! !: typeclass_instances. *)
 (* Elpi add_instances Inj ignoreInstances compose_inj. *)
 (* Elpi add_instances instances compose_inj isInjf_eq isInjg_eq. *)
 (* Elpi add_instances instances inr_inj. *)
-
-Goal forall (A: Type) (x: A -> A), let y := Inj eq eq x in let z := y in z -> Inj eq eq (compose x x).
-Proof.
-  intros T x y z H.
-  (* following diverges: the compiler should unfold the def *)
-  (* Check (_ : Inj eq eq (compose x x)). *)
-Admitted. 
