apps/tc/tc/myEqDec/eqDecSimpl.v
@@ -1,0 +1,64 @@
+Require Export Bool Arith List.
+From Coq Require Import FunctionalExtensionality.
+
+Export ListNotations.
+Generalizable Variables A B.
+
+Class Eqb A : Type := eqb : A -> A -> bool.
+
+Notation " x == y " := (eqb x y) (no associativity, at level 70).
+
+Definition neqb {A} `{Eqb A} (x y : A) := negb (x == y). 
+
+Local Instance eqU : Eqb unit := { eqb x y := true }.
+Local Instance eqB : Eqb bool := { eqb x y := if x then y else negb y }.
+Local Instance eqP {A B} `{Eqb A} `{Eqb B} : Eqb (A * B) := { 
+  eqb x y := (fst x == fst y) && (snd x == snd y) }.
+
+(* Set Typeclasses Debug. *)
+
+From elpi Require Import elpi.
+From elpi.apps Require Export tc.compiler.
+Elpi Override TC TC_check Eqb.
+(* Elpi add_instances EqDec. *)
+
+Elpi Accumulate TC_check lp:{{
+  tc {{ Eqb unit }} {{ eqU }}.
+  tc {{ Eqb bool }} {{ eqB }}.
+  tc {{ Eqb (prod lp:A lp:B) }} {{ @eqP _ _ lp:EqA lp:EqB }} :- 
+    tc {{ Eqb lp:A }} EqA,
+    tc {{ Eqb lp:B }} EqB.
+}}.
+Elpi Print TC_check.
+
+Check ((tt, (tt, true)) == (tt, (tt, true))).
+Check (1 == 2).
+Compute (fst (1, 2)).
+
+Local Instance eq_nat : EqDec nat := {
+  eqb := fix aux i1 i2 := 
+  match i1, i2 return bool with
+    | O, O => true 
+    | S x, S y => aux x y
+    | _, _ => false 
+  end 
+}.
+Local Instance eq_list `(eqa : (EqDec A)) : EqDec (list A) :=
+  { eqb := fix aux (x y : list A) :=
+    match x, y return bool with
+    | [], [] => true 
+    | x :: xs, y :: ys => (eqb x y) && (aux xs ys)
+    | _, _ => false
+    end }.
+Local Instance eq_bool_to_bool `(EqDec A) : EqDec (bool -> A) :=
+{
+  eqb f g := (f true == g true) && (f false == g false)
+}.
+Proof.
+  intros x y Hyp.
+  (* Search _ inside FunctionalExtensionality. *)
+  apply functional_extensionality.
+  rewrite andb_true_iff in Hyp.
+  intros [].
+  all : now apply (eqb_leibniz (x _) (y _)).
+Defined.
