apps/tc/tc/stdpp/exampleBugGlobInst.v
@@ -1,0 +1,18 @@
+From elpi.apps.tc Require Import compiler.
+From Coq Require Export Setoid.
+
+Generalizable All Variables.
+
+Class Inj {A B} (R : relation A) (S : relation B) (f : A -> B) : Prop :=
+  inj x y : S (f x) (f y) -> R x y.
+
+Section testInj.
+  Context {A : Type}.
+  Global Instance xxx : Inj eq eq (@id A). Admitted.
+  Elpi add_instances Inj.
+  Elpi Print TC_check.
+End testInj.
+Elpi Print TC_check.
+
+Print Instances Inj.
+Elpi print_instances.
